Batteries/Data/RBMap/Lemmas.lean
@@ -43,7 +43,7 @@ theorem mem_congr [Ord α] [@TransCmp α compare] {t : RBNode α} (h : compare x
     Mem x t ↔ Mem y t := by simp [Mem, TransCmp.cmp_congr_left' h]
 
 theorem isOrdered_iff' [@TransCmp α cmp] {t : RBNode α} :
-    isOrdered cmp t L R ↔
+    @isOrdered α ⟨cmp⟩ t L R ↔
     (∀ a ∈ L, t.All (cmpLT cmp a ·)) ∧
     (∀ a ∈ R, t.All (cmpLT cmp · a)) ∧
     (∀ a ∈ L, ∀ b ∈ R, cmpLT cmp a b) ∧
@@ -65,7 +65,7 @@ theorem isOrdered_iff' [@TransCmp α cmp] {t : RBNode α} :
         ⟨vr, fun _ h => (hR _ h).2.2, fun _ h => (hR _ h).1, or⟩⟩⟩
 
 theorem isOrdered_iff [@TransCmp α cmp] {t : RBNode α} :
-    isOrdered cmp t ↔ @Ordered α ⟨cmp⟩ t := by simp [isOrdered_iff']
+    @isOrdered α ⟨cmp⟩ t none none ↔ @Ordered α ⟨cmp⟩ t := by simp [isOrdered_iff']
 
 instance (cmp) [@TransCmp α cmp] (t) : Decidable (@Ordered α ⟨cmp⟩ t) := decidable_of_iff _ isOrdered_iff
 
